test/rcases.lean
@@ -22,6 +22,7 @@ example (x : α × β × γ) : true :=
 begin
   rcases x with ⟨a, ⟨-, c⟩⟩,
   { guard_hyp a := α,
+    success_if_fail { guard_hyp x_snd_fst := β },
     guard_hyp c := γ,
     trivial }
 end
@@ -65,6 +66,7 @@ begin
   { existsi 0, simp },
   guard_hyp n := ℕ,
   guard_hyp h := n = n,
+  success_if_fail {assumption},
   trivial
 end
 
@@ -130,4 +132,27 @@ example (n : ℕ) : true :=
 begin
   obtain one_lt_n | (n_le_one : n + 1 ≤ 1) := nat.lt_or_ge 1 (n + 1),
   trivial, trivial,
+end
+
+example (h : ∃ x : ℕ, x = x ∧ 1 = 1) : true :=
+begin
+  rcases h with ⟨-, _⟩,
+  (do lc ← tactic.local_context, guard lc.empty),
+  trivial
+end
+
+example (h : ∃ x : ℕ, x = x ∧ 1 = 1) : true :=
+begin
+  rcases h with ⟨-, _, h⟩,
+  (do lc ← tactic.local_context, guard (lc.length = 1)),
+  guard_hyp h := 1 = 1,
+  trivial
+end
+
+example (h : true ∨ true ∨ true) : true :=
+begin
+  rcases h with -|-|-,
+  iterate 3 {
+    (do lc ← tactic.local_context, guard lc.empty),
+    trivial },
 end
